Fix the bugs introduced when splitting the translation between several files. Clean up.

candle/standard/cf_kernel/ml_hol_kernelProgScript.sml
@@ -1,307 +1,247 @@
-open preamble
-open astTheory libTheory semanticPrimitivesTheory bigStepTheory
-     ml_translatorTheory ml_translatorLib ml_progTheory ml_progLib
-     ml_pmatchTheory holKernelTheory ml_monadBaseTheory ml_monadProgTheory
-open terminationTheory
-open ml_monadStoreLib ml_hol_kernelStoreProgTheory
+open preamble ml_translatorTheory ml_translatorLib ml_pmatchTheory patternMatchesTheory
+open astTheory libTheory bigStepTheory semanticPrimitivesTheory
+open terminationTheory ml_progLib ml_progTheory
+open set_sepTheory cfTheory cfStoreTheory cfTacticsLib Satisfy
+open cfHeapsBaseTheory basisFunctionsLib
+open ml_monadBaseTheory ml_monadProgTheory ml_monadStoreLib ml_monad_translatorLib holKernelTheory
 
 val _ = new_theory "ml_hol_kernelProg";
-
-val RW = REWRITE_RULE;
-val RW1 = ONCE_REWRITE_RULE;
-
-val _ = (print_asts := true);
-
-val _ = translation_extends "ml_hol_kernelStoreProg"
-
+			
 val _ = (use_full_type_names := false);
 
-(* PROVISIONAL *)
-val _ = type_abbrev("M", ``:'a -> ('b, 'c) exc # 'a``);
-(* END OF PROVISIONAL *)
+val _ = register_type ``:cpn``
+val _ = register_type ``:'a # 'b``;
+val _ = register_type ``:'a list``
+val _ = register_type ``:'a option``
 
-fun dest_monad_type ty =
-  let val s = (match_type ``:('a, 'b, 'c) M`` ty) in
-      (type_subst s ``:'a``, type_subst s ``:'b``, type_subst s ``:'c``) end;
+val _ = ml_prog_update (open_module "Kernel");
 
-(* Should be moved somewhere else *)
-fun list_dest f tm =
-  let val (x,y) = f tm in list_dest f x @ list_dest f y end
-  handle HOL_ERR _ => [tm];
-val dest_fun_type = dom_rng
-fun domain ty = ty |> dest_fun_type |> fst
+val _ = temp_type_abbrev("state",``:'ffi semanticPrimitives$state``);
 
-fun dest_args tm =
-  let val (x,y) = dest_comb tm in dest_args x @ [y] end
-  handle HOL_ERR _ => []
+(* construct type refinement invariants *)
 
-fun D th = let
-  val th = th |> DISCH_ALL |> PURE_REWRITE_RULE [AND_IMP_INTRO]
-  in if is_imp (concl th) then th else DISCH T th end
+val _ = register_type ``:type``;
 
-val env_tm = mk_var("env",semanticPrimitivesSyntax.mk_environment semanticPrimitivesSyntax.v_ty)
+val MEM_type_size = Q.prove(
+  `!ts t. MEM t ts ==> type_size t < type1_size ts`,
+  Induct \\ FULL_SIMP_TAC (srw_ss()) [] \\ REPEAT STRIP_TAC \\ RES_TAC
+  \\ EVAL_TAC \\ FULL_SIMP_TAC std_ss [] \\ DECIDE_TAC);
 
-(* Theorems, predicates and types valid for the current translation *)
-(* val H = ``HOL_STORE``;
-val refs_type = type_of H |> dest_type |> snd |> List.hd;
-fun M_type ty = ``:(hol_refs, ^ty, hol_exn) M``;
-val aM = ty_antiq (M_type ``:'a``);
-val bM = ty_antiq (M_type ``:'b``);
+val type_ind = Q.store_thm("type_ind",
+  `(!s ts. (!t. MEM t ts ==> P t) ==> P (Tyapp s ts)) /\
+    (!v. P (Tyvar v)) ==> !x. P x`,
+  REPEAT STRIP_TAC \\ completeInduct_on `type_size x`
+  \\ REPEAT STRIP_TAC \\ FULL_SIMP_TAC std_ss [PULL_FORALL]
+  \\ Cases_on `x` \\ FULL_SIMP_TAC std_ss []
+  \\ Q.PAT_X_ASSUM `!x1 x2. bb` MATCH_MP_TAC
+  \\ REPEAT STRIP_TAC \\ Q.PAT_X_ASSUM `!x.bbb` MATCH_MP_TAC
+  \\ EVAL_TAC \\ IMP_RES_TAC MEM_type_size \\ DECIDE_TAC);
 
-val VALID_STORE_THM = HOL_STORE_EXISTS;
-val EXN_TYPE = ``HOL_EXN_TYPE``;
-val exn_type = type_of EXN_TYPE |> dest_type |> snd |> List.hd
-val additional_theories = ["ml_hol_kernelStoreProg"]; *)
+val TYPE_TYPE_def = fetch "-" "TYPE_TYPE_def"
 
-(* The store predicate *) 
-val H = ref ``\refs. emp``;
+val LIST_TYPE_NO_CLOSURES = Q.prove(
+  `!xs v.
+      (!x v. MEM x xs /\ p x v ==> no_closures v) /\
+      LIST_TYPE p xs v ==> no_closures v`,
+  Induct \\ FULL_SIMP_TAC std_ss [LIST_TYPE_def]
+  \\ REPEAT STRIP_TAC \\ FULL_SIMP_TAC std_ss [no_closures_def,EVERY_DEF,MEM]
+  \\ METIS_TAC []);
 
-(* The type of the references object *)
-val refs_type = ref ``:unit``;
+val LIST_TYPE_11 = Q.prove(
+  `!P ts v1 us v2.
+      (!x1.
+       MEM x1 ts ==>
+        !v1 x2 v2.
+          P x1 v1 /\ P x2 v2 ==>
+          types_match v1 v2 /\ ((v1 = v2) <=> (x1 = x2))) /\
+    LIST_TYPE P ts v1 /\ LIST_TYPE P us v2 ==>
+    types_match v1 v2 /\ ((v1 = v2) = (ts = us))`,
+  STRIP_TAC \\ Induct \\ Cases_on `us` \\ FULL_SIMP_TAC (srw_ss()) []
+  \\ SIMP_TAC (srw_ss()) [LIST_TYPE_def,types_match_def,ctor_same_type_def]
+  \\ FULL_SIMP_TAC (srw_ss()) [PULL_EXISTS,types_match_def,ctor_same_type_def]
+  \\ METIS_TAC []);
 
-(* The exception refinement invariant and type *)
-val EXN_TYPE = ref ``UNIT_TYPE``;
-val exn_type = ref ``:unit``;
+val CHAR_IMP_no_closures = Q.prove(
+  `CHAR x v ==> no_closures v`,
+  SIMP_TAC std_ss [CHAR_def,no_closures_def]);
 
-(* Some functions to generate monad types *)
-fun M_type ty = ``:(^(!refs_type), ^ty, ^(!exn_type)) M``;
-val aM = ref (ty_antiq (M_type ``:'a``));
-val bM = ref (ty_antiq (M_type ``:'b``));
+val STRING_IMP_no_closures = Q.prove(
+  `STRING_TYPE x v ==> no_closures v`,
+  Cases_on`x` \\ SIMP_TAC std_ss [STRING_TYPE_def,no_closures_def]);
 
-(* The theorem stating that there exists a store stasfying the store predicate *)
-val VALID_STORE_THM = ref (prove(``T``, fs[]));
+val EqualityType_thm = Q.prove(
+  `EqualityType abs <=>
+      (!x1 v1. abs x1 v1 ==> no_closures v1) /\
+      (!x1 v1 x2 v2. abs x1 v1 /\ abs x2 v2 ==> types_match v1 v2 /\
+                                                (v1 = v2 <=> x1 = x2))`,
+  SIMP_TAC std_ss [EqualityType_def] \\ METIS_TAC []);
 
-(* Additional theories where to look for refinement invariants *)
-val additional_theories = ref ([] : string list);
+val STRING_TYPE_lemma = Q.prove(
+  `EqualityType (STRING_TYPE)`,
+  METIS_TAC (eq_lemmas ()));
 
-(* Theorems proved by the user to handle exceptions *)
-val custom_patterns = ref ([] : thm list);
+val EqualityType_TYPE = Q.prove(
+  `EqualityType TYPE_TYPE`,
+  SIMP_TAC std_ss [EqualityType_thm] \\ STRIP_TAC THEN1
+   (HO_MATCH_MP_TAC type_ind
+    \\ FULL_SIMP_TAC std_ss [TYPE_TYPE_def]
+    \\ REPEAT STRIP_TAC
+    \\ FULL_SIMP_TAC std_ss [no_closures_def,EVERY_DEF]
+    \\ IMP_RES_TAC (LIST_TYPE_NO_CLOSURES |> GEN_ALL)
+    \\ METIS_TAC [CHAR_IMP_no_closures,STRING_IMP_no_closures])
+  \\ HO_MATCH_MP_TAC type_ind \\ reverse STRIP_TAC THEN1
+   (REPEAT STRIP_TAC
+    \\ Cases_on `x2` \\ FULL_SIMP_TAC (srw_ss()) [TYPE_TYPE_def]
+    \\ FULL_SIMP_TAC (srw_ss()) [types_match_def,ctor_same_type_def]
+    \\ ASSUME_TAC STRING_TYPE_lemma
+    \\ FULL_SIMP_TAC std_ss [EqualityType_def] \\ RES_TAC)
+  \\ REPEAT GEN_TAC \\ STRIP_TAC \\ REPEAT GEN_TAC \\ STRIP_TAC
+  \\ Cases_on `x2` \\ FULL_SIMP_TAC (srw_ss()) [TYPE_TYPE_def]
+  \\ FULL_SIMP_TAC (srw_ss()) [types_match_def,ctor_same_type_def]
+  \\ MATCH_MP_TAC (METIS_PROVE [] ``(b1 /\ (x1 = y1)) /\ (b2 /\ (x2 = y2)) ==>
+       (b1 /\ b2) /\ ((x1 /\ x2 <=> y1 /\ y2))``)
+  \\ STRIP_TAC THEN1
+   (ASSUME_TAC STRING_TYPE_lemma
+    \\ FULL_SIMP_TAC std_ss [EqualityType_def] \\ RES_TAC
+    \\ ASM_SIMP_TAC std_ss [])
+  \\ MATCH_MP_TAC LIST_TYPE_11
+  \\ Q.EXISTS_TAC `TYPE_TYPE`
+  \\ FULL_SIMP_TAC std_ss []
+  \\ REPEAT STRIP_TAC \\ RES_TAC)
+  |> store_eq_thm;
 
+val _ = register_type ``:term``;
+val _ = register_type ``:thm``;
+val _ = register_type ``:update``;
+val _ = register_exn_type ``:hol_exn``;
 
-(* Initialize the translation by giving the appropriate values to the above references *)
-fun init_translation (store_trans_res : store_translation_result) custom_patterns type_theories =
-  let
-      val {init_values_thms = init_values_thms,
-	   locations_thms  = locations_thms,
-	   store_pred_def = store_pred_def,
-	   store_pred_validity = store_pred_validity,
-	   store_pred_exists_thm = store_pred_exists_thm,
-	   get_specs = get_specs,
-	   set_specs = set_specs} = store_trans_res
-      val _ = (H := concl store_pred_def |> des_eq |> fst)
-      val _ = (refs_type := dest_type (!H) |> snd |> List.hd)
-      val _ = (EXN_TYPE := List.hd get_specs |> concl |> dest_imp |> snd |> rator |> rand |> rator |> rator)
-      val _ = (aM := (ty_antiq (M_type ``:'a``)))
-      val _ = (bM := (ty_antiq (M_type ``:'b``)))
-      val _ = (VALID_STORE_THM := store_pred_exists_thm)
-      val _ = (additional_theories := type_theories)
-      val _ = (custom_patterns := custom_patterns)
-  in () end;
+val HOL_EXN_TYPE_def = theorem"HOL_EXN_TYPE_def";
 
-val t= (1 |-> 2)
-val {redex = x, residue = y} = t;
+(* Prove the specifications for the exception handling *)
 
-val spec = ``nsLookup env.v (Short ^name_tm) = SOME ^loc_const ==>
-            EvalM env (App Opderef [Var (Short ^name_tm)])
-            (^MONAD_RI ^monad_get_fun) ^store_pred``
+(* failwith *)
+val EvalM_failwith = Q.store_thm("EvalM_failwith",
+  `!H x a.
+      (lookup_cons "Fail" env = SOME (1,TypeExn (Long "Kernel" (Short "Fail")))) ==>
+      Eval env exp1 (STRING_TYPE x) ==>
+      EvalM env (Raise (Con (SOME (Short "Fail")) [exp1]))
+        (MONAD a HOL_EXN_TYPE (failwith x)) H`,
+  rw[Eval_def,EvalM_def,MONAD_def,failwith_def] >>
+  rw[Once evaluate_cases] >>
+  rw[Once evaluate_cases] >>
+  srw_tac[boolSimps.DNF_ss][] >> disj1_tac >>
+  rw[Once evaluate_cases,PULL_EXISTS] >>
+  rw[Once(CONJUNCT2 evaluate_cases)] >>
+  first_x_assum(qspec_then`(s with refs := s.refs ++ junk).refs`strip_assume_tac) >>
+  IMP_RES_TAC (evaluate_empty_state_IMP
+               |> INST_TYPE [``:'ffi``|->``:unit``]) >>
+  rw[do_con_check_def,build_conv_def] >>
+  fs [lookup_cons_def] >>
+  fs[HOL_EXN_TYPE_def,namespaceTheory.id_to_n_def] >>
+  asm_exists_tac \\ fs[] >>
+  PURE_REWRITE_TAC[GSYM APPEND_ASSOC] \\ METIS_TAC[REFS_PRED_append]);
 
-type store_translation_thms =
-    {init_values_thms : thm list,
-     locations_thms  : thm list,
-     store_pred_def : thm,
-     store_pred_validity : thm,
-     store_pred_exist_thm : thm,
-     get_specs : thm list,
-     set_specs : thm list};
+(* clash *)
 
-fun mk_store_translation_thms values locs pred pred_valid pred_exists gets sets =
-   ({init_values_thms = values,
-     locations_thms  = locs,
-     store_pred_def = pred,
-     store_pred_validity = pred_valid,
-     store_pred_exist_thm = pred_exists,
-     get_specs = gets,
-     set_specs = sets} : store_translation_thms);
+val EvalM_raise_clash = Q.store_thm("EvalM_raise_clash",
+  `!H x a.
+      (lookup_cons "Clash" env = SOME (1,TypeExn (Long "Kernel" (Short "Clash")))) ==>
+      Eval env exp1 (TERM_TYPE x) ==>
+      EvalM env (Raise (Con (SOME (Short "Clash")) [exp1]))
+        (MONAD a HOL_EXN_TYPE (raise_clash x)) H`,
+  rw[Eval_def,EvalM_def,MONAD_def,raise_clash_def] >>
+  rw[Once evaluate_cases] >>
+  rw[Once evaluate_cases] >>
+  srw_tac[boolSimps.DNF_ss][] >> disj1_tac >>
+  rw[Once evaluate_cases,PULL_EXISTS] >>
+  rw[Once(CONJUNCT2 evaluate_cases)] >>
+  rw[do_con_check_def,build_conv_def] >>
+  fs [lookup_cons_def] >>
+  fs[HOL_EXN_TYPE_def,namespaceTheory.id_to_n_def] >>
+  first_x_assum(qspec_then`(s with refs := s.refs ++ junk).refs`strip_assume_tac) >>
+  IMP_RES_TAC (evaluate_empty_state_IMP
+               |> INST_TYPE [``:'ffi``|->``:unit``]) >>
+  fs[] >> asm_exists_tac \\ fs[] >>
+  PURE_REWRITE_TAC[GSYM APPEND_ASSOC] \\ METIS_TAC[REFS_PRED_append]);
 
-val ISPEC_EvalM = ISPEC (!H);
-val ISPEC_EvalM_MONAD = ISPECL[!H, !EXN_TYPE];
+(* handle_clash *)
 
-fun inst_monad_type tm =
-  let
-      val ty_subst = Type.match_type ``:('a, 'b, 'c) M`` (type_of tm)
-      val a = Type.type_subst ty_subst ``:'a``
-      val c = Type.type_subst ty_subst ``:'c``
-      val tm' = Term.inst [a |-> refs_type, c |-> exn_type] tm
-  in
-      tm'
-  end;
-(* ---- *)
+val EvalM_handle_clash = Q.store_thm("EvalM_handle_clash",
+  `!H n. (lookup_cons "Clash" env = SOME (1,TypeExn (Long "Kernel" (Short "Clash")))) ==>
+        EvalM env exp1 (MONAD a HOL_EXN_TYPE x1) H ==>
+        (!t v.
+          TERM_TYPE t v ==>
+          EvalM (write n v env) exp2 (MONAD a HOL_EXN_TYPE (x2 t)) H) ==>
+        EvalM env (Handle exp1 [(Pcon (SOME (Short "Clash")) [Pvar n],exp2)])
+          (MONAD a HOL_EXN_TYPE (handle_clash x1 x2)) H`,
+  SIMP_TAC std_ss [EvalM_def] \\ REPEAT STRIP_TAC
+  \\ SIMP_TAC (srw_ss()) [Once evaluate_cases]
+  \\ Q.PAT_X_ASSUM `!s refs. REFS_PRED H refs s ==> bbb` (MP_TAC o Q.SPECL [`s`,`refs`])
+  \\ FULL_SIMP_TAC std_ss [] \\ REPEAT STRIP_TAC
+  \\ first_x_assum(qspec_then`junk`strip_assume_tac)
+  \\ Cases_on `res` THEN1
+   (srw_tac[DNF_ss][] >> disj1_tac \\
+    asm_exists_tac \\ fs[MONAD_def,handle_clash_def] \\
+    CASE_TAC \\ fs[] \\ CASE_TAC \\ fs[] )
+  \\ Q.PAT_X_ASSUM `MONAD xx yy zz t1 t2` MP_TAC
+  \\ SIMP_TAC std_ss [Once MONAD_def] \\ STRIP_TAC
+  \\ Cases_on `x1 refs` \\ FULL_SIMP_TAC (srw_ss()) []
+  \\ Cases_on `q` \\ FULL_SIMP_TAC (srw_ss()) [handle_clash_def]
+  \\ Cases_on `e` \\ FULL_SIMP_TAC (srw_ss()) [handle_clash_def]
+  \\ srw_tac[boolSimps.DNF_ss][] >> disj2_tac >> disj1_tac
+  \\ asm_exists_tac \\ fs[]
+  \\ simp[Once (CONJUNCT2 evaluate_cases),PULL_EXISTS,pat_bindings_def]
+  \\ Cases_on `b` >> fs[HOL_EXN_TYPE_def] >>
+  simp[pmatch_def] >> fs[lookup_cons_def] >>
+  fs[same_tid_def,namespaceTheory.id_to_n_def,same_ctor_def] >- (
+    simp[Once evaluate_cases,MONAD_def,HOL_EXN_TYPE_def] ) >>
+  first_x_assum drule >>
+  disch_then drule >>
+  simp[GSYM write_def] >>
+  disch_then(qspec_then`[]`strip_assume_tac) >>
+  fs[with_same_refs] >>
+  asm_exists_tac >>
+  fs[MONAD_def] >>
+  TOP_CASE_TAC \\ fs[] \\
+  TOP_CASE_TAC \\ fs[] \\
+  TOP_CASE_TAC \\ fs[] \\
+  TOP_CASE_TAC \\ fs[]);
 
-(* ---- *)
-(* TODO: move HOL_MONAD_tm *)
-val MONAD_POLY_tm = ``MONAD : ('a -> v -> bool) -> ('b -> v -> bool) -> (('refs, 'a, 'b) M, 'refs) H``;
-val MONAD_tm = Term.inst [``:'refs`` |-> refs_type] MONAD_POLY_tm;
-fun get_m_type_inv ty =
-  let
-      val monad_type = dest_monad_type ty |> #2
-      val MONAD_tm' = Term.inst [``:'a`` |-> monad_type, ``:'b`` |-> exn_type] MONAD_tm
-  in
-      ``^MONAD_tm' ^(get_type_inv monad_type) ^EXN_TYPE``
-  end
-  handle HOL_ERR _ => failwith "unknown type";
+val exn_thms = [EvalM_failwith, EvalM_raise_clash, EvalM_handle_clash];
 
-val PURE_tm = ``PURE : ('a -> v -> bool) -> ('a, 'b) H``;
-fun mk_PURE_tm ty = let
-  val PURE_tm' = Term.inst [``:'a`` |-> ty, ``:'b`` |-> refs_type] PURE_tm
-  in mk_comb (PURE_tm', get_type_inv ty) end;
+(* Define and translate the store *)
+val init_type_constants_def = Define `
+init_type_constants = [(strlit"bool",0); (strlit"fun",2:num)]`;
 
-fun get_arrow_type_inv ty =
-  if can dest_monad_type ty then get_m_type_inv ty else let
-    val (ty1,ty2) = dest_fun_type ty
-    val i1 = get_arrow_type_inv ty1 handle HOL_ERR _ =>
-             mk_PURE_tm ty1
-             (* ``PURE ^(get_type_inv ty1)`` *)
-    val i2 = get_arrow_type_inv ty2
-    in ``ArrowM ^H ^i1 ^i2`` end
+val init_term_constants_def = Define `
+  init_term_constants = [(strlit"=",
+    Tyapp (strlit"fun")
+      [Tyvar (strlit"A");
+       Tyapp (strlit"fun")
+         [Tyvar (strlit"A");
+          Tyapp (strlit"bool") []]])]`;
 
-fun smart_get_type_inv ty =
-  if not (can dest_monad_type ty) andalso
-     can get_arrow_type_inv ty then let
-    val inv = get_arrow_type_inv ty
-    in ONCE_REWRITE_CONV [ArrowM_def] inv |> concl |> rand |> rand end
-  else get_type_inv ty
+val init_axioms_def = Define `
+  init_axioms = []:thm list`;
 
-(* Retrieves the parameters given to Eval or EvalM *)
-val Eval_tm = ``Eval``;
-val EvalM_tm = ``EvalM``;
-fun get_Eval_arg e = if same_const (strip_comb e |> fst) Eval_tm then e |> rand |> rand
-		     else e |> rator |> rand |> rand;
-fun get_Eval_env e = if same_const (strip_comb e |> fst) Eval_tm then e |> rator |> rator |> rand
-		     else e |> rator |> rator |> rator |> rand;
-fun get_Eval_exp e = if same_const (strip_comb e |> fst) Eval_tm then e |> rator |> rand
-		     else e |> rator |> rator |> rand;
-fun remove_Eval_storePred e = if same_const (strip_comb e |> fst) Eval_tm then e
-		     else e |> rator;
-(* ---- *)
+val init_context_def = Define `
+  init_context = ^(rhs(concl(holSyntaxTheory.init_ctxt_def)))`;
 
-(* support for datatypes... *)
+val refs_init_list = [
+  ("the_type_constants", init_type_constants_def, get_the_type_constants_def,
+  set_the_type_constants_def),
+  ("the_term_constants", init_term_constants_def, get_the_term_constants_def,
+  set_the_term_constants_def),
+  ("the_axioms", init_axioms_def, get_the_axioms_def, set_the_axioms_def),
+  ("the_context", init_context_def, get_the_context_def, set_the_context_def)
+];
 
-(*
-val ty = ``:'b # 'c``; val th = derive_case_of ty;
-val ty = ``:'a list``; val th = derive_case_of ty;
-val ty = ``:type``; val th = derive_case_of ty;
-val ty = ``:term``; val th = derive_case_of ty;
-val ty = ``:thm``; val th = derive_case_of ty;
-val ty = ``:update``; val th = derive_case_of ty;
-*)
+val store_hprop_name = "HOL_STORE";
+val exc_ri = ``HOL_EXN_TYPE``;
+val translated_store_thms = translate_store refs_init_list store_hprop_name exc_ri;
 
-(******************************************************************************************
- *
- * Pattern matching
- *
- ******************************************************************************************)
-
-(*
-  val _ = set_goal([],goal)
-*)	      
-fun derive_case_of ty = let
-  fun smart_full_name_of_type ty =
-    if let val r = dest_thy_type ty in #Tyop r = "cpn" andalso #Thy r = "toto" end then "order"
-    else full_name_of_type ty
-  fun get_name ty = clean_uppercase (smart_full_name_of_type ty) ^ "_TYPE"
-  val name = get_name ty
-  val inv_def = tryfind (fn thy_name => fetch thy_name (name ^ "_def"))
-                        (current_theory()::(additional_theories@ [(*"ml_monadProg",*) "ml_translator"]))
-  val case_th = get_nchotomy_of ty
-(*
-  val tm = ``Eval (write n1_2 v1_2 (write n1_1 v1_1 env)) exp1
-      (return_type (f1 x1_1 x1_2))``
-*)
-  val pat = ``Eval env exp (P (res:'a))``
-  (* TODO: Add support for H, add type of refs in `'a M` *)
-  fun Eval_to_EvalM tm = let
-    val (m,i) = match_term pat tm
-    val res = mk_var("res", M_type ``:'a``)
-    val tm1 = subst m (inst i ``EvalM env exp (MONAD P ^EXN_TYPE ^res) ^H``)
-    val ty1 = tm |> rand |> rand |> type_of
-    val monad_ret_type = M_type ty1(* type_subst [``:'a`` |-> ty1] monad_type1 *)
-    val y1 = tm |> rand |> rand |> inst [ty1|->monad_ret_type]
-    val y0 = tm1 |> rator |> rand |> rand
-    in subst [y0 |-> y1] tm1 end
-    handle HOL_ERR _ =>
-    if is_comb tm then let
-      val (x,y) = dest_comb tm
-      in mk_comb(Eval_to_EvalM x, Eval_to_EvalM y) end
-    else if is_abs tm then let
-      val (x,y) = dest_abs tm
-      in mk_abs(x, Eval_to_EvalM y) end
-    else tm
-  val pure_tm = case_of ty |> concl
-  val (x1,x2) = dest_imp pure_tm
-  val (x2,x3) = dest_imp x2
-  val (x3,x4) = dest_imp x3
-  (* val tm = last hyps |> strip_forall |> snd |> dest_imp |> snd *)
-  val hyps = list_dest dest_conj x3
-  fun map_tl f [] = []
-    | map_tl f (x::xs) = x :: map f xs
-  val z3 = map_tl Eval_to_EvalM hyps |> list_mk_conj
-  val z4 = Eval_to_EvalM x4
-  val goal = mk_imp(x1,mk_imp(x2,mk_imp(z3,z4)))
-  val evaluate_Mat =
-    ``evaluate c x env (Mat e pats) (xx,res)``
-    |> (ONCE_REWRITE_CONV [evaluate_cases] THENC SIMP_CONV (srw_ss()) [])
-  val evaluate_match_Conv =
-    ``evaluate_match c x env args
-         ((Pcon xx pats,exp2)::pats2) errv (yyy,y)``
-    |> (ONCE_REWRITE_CONV [evaluate_cases] THENC
-        SIMP_CONV (srw_ss()) [pmatch_def])
-  val IF_T = Q.prove(`(if T then x else y) = x:'a`,SIMP_TAC std_ss []);
-  val IF_F = Q.prove(`(if F then x else y) = y:'a`,SIMP_TAC std_ss []);
-  val init_tac =
-        PURE_REWRITE_TAC [CONTAINER_def]
-        \\ REPEAT STRIP_TAC \\ STRIP_ASSUME_TAC (Q.SPEC `x` case_th)
-  val case_tac =
-        Q.PAT_X_ASSUM `b0 ==> Eval env exp something`
-           (MP_TAC o REWRITE_RULE [TAG_def,inv_def,Eval_def])
-        \\ FULL_SIMP_TAC (srw_ss()) []
-        \\ REPEAT STRIP_TAC
-        \\ NTAC 2 (POP_ASSUM MP_TAC)
-        \\ POP_ASSUM (STRIP_ASSUME_TAC o remove_primes o
-             SPEC_ALL o REWRITE_RULE [TAG_def,inv_def,EvalM_def])
-        \\ FULL_SIMP_TAC std_ss [ALL_DISTINCT] \\ FULL_SIMP_TAC std_ss [inv_def]
-        \\ REPEAT STRIP_TAC
-        \\ FULL_SIMP_TAC std_ss [ALL_DISTINCT] \\ FULL_SIMP_TAC std_ss [inv_def]
-        \\ FULL_SIMP_TAC std_ss [EvalM_def,PULL_FORALL] \\ REPEAT STRIP_TAC
-        \\ ONCE_REWRITE_TAC [evaluate_cases] \\ SIMP_TAC (srw_ss()) []
-        \\ SIMP_TAC (std_ss ++ DNF_ss) [] \\ disj1_tac
-        \\ first_x_assum(qspec_then`(s with refs := s.refs ++ junk).refs`strip_assume_tac)
-        \\ drule evaluate_empty_state_IMP
-        \\ strip_tac \\ asm_exists_tac
-        \\ ASM_SIMP_TAC std_ss []
-        \\ REWRITE_TAC[evaluate_match_Conv,pmatch_def,LENGTH]
-        \\ fs[pmatch_def,pat_bindings_def,write_def,
-              lookup_cons_def,same_tid_def,namespaceTheory.id_to_n_def,same_ctor_def]
-        \\ ONCE_REWRITE_TAC[GSYM APPEND_ASSOC]
-        \\ first_x_assum (match_mp_tac o MP_CANON)
-        \\ fs[]
-(*
-  val _ = set_goal([],goal)
-*)
-  val tac = init_tac THEN case_tac
-  val case_lemma = prove(goal,tac)
-  val case_lemma = case_lemma |> PURE_REWRITE_RULE [TAG_def]
-  in case_lemma end;
-
-fun type_mem f = let
-  val memory = ref []
-  fun lookup x [] = fail()
-    | lookup x ((y,z)::ys) = if can (match_type y) x then z else lookup x ys
-  in fn ty => lookup ty (!memory) handle HOL_ERR _ => let
-              val th = f ty
-              val _ = (memory := (ty,th)::(!memory))
-              in th end end;
-
-val mem_derive_case_of = type_mem derive_case_of;
+(* Initialize the monadic translation *)
+val _ = init_translation translated_store_thms exn_thms []
 
 val ty = ``:'b # 'c``; val _ = mem_derive_case_of ty;
 val ty = ``:'a list``; val _ = mem_derive_case_of ty;
@@ -311,810 +251,8 @@ val ty = ``:term``; val _ = mem_derive_case_of ty;
 val ty = ``:thm``; val _ = mem_derive_case_of ty;
 val ty = ``:update``; val _ = mem_derive_case_of ty;
 
-(*
-val tm = ``case l of [] => ex_return F | x::l' => ex_return T``;
-inst_case_thm_for tm;
-*)
-
-fun inst_case_thm_for tm = let
-  val (_,_,names) = TypeBase.dest_case tm
-  val names = map fst names
-  val th = mem_derive_case_of ((repeat rator tm) |> type_of |> domain) |> UNDISCH
-  val pat = th |> UNDISCH_ALL |> concl |> rator |> rand |> rand
-  val (ss,i) = match_term pat tm
-  val th = INST ss (INST_TYPE i th)
-  val ii = map (fn {redex = x, residue = y} => (x,y)) i
-  val ss = map (fn (x,y) => (inst i (smart_get_type_inv x) |-> smart_get_type_inv y)) ii
-  val th = INST ss th
-  val th = CONV_RULE (DEPTH_CONV BETA_CONV) th
-  fun args tm = let val (x,y) = dest_comb tm in args x @ [y] end
-                handle HOL_ERR _ => []
-  val ns = map (fn n => (n,args n)) names
-  fun rename_var prefix ty v =
-    mk_var(prefix ^ implode (tl (explode (fst (dest_var v)))),ty)
-  val ts = find_terms (can (match_term ``ml_translator$CONTAINER (b:bool)``)) (concl th)
-           |> map (rand o rand)
-           |> map (fn tm => (tm,map (fn x => (x,rename_var "n" ``:string`` x,
-                                                rename_var "v" ``:v`` x))
-                    (dest_args tm handle HOL_ERR _ => [])))
-  val ns = map (fn (tm,xs) => let
-      val aa = snd (first (fn (pat,_) => can (match_term tm) pat) ns)
-      in zip aa xs end) ts |> flatten
-  val ms = map (fn (b,(x,n,v)) => n |-> stringSyntax.fromMLstring (fst (dest_var b))) ns
-  val th = INST ms th
-  val ks = map (fn (b,(x,n,v)) => (fst (dest_var x), fst (dest_var b))) ns @
-           map (fn (b,(x,n,v)) => (fst (dest_var v), fst (dest_var b) ^ "{value}")) ns
-  fun rename_bound_conv tm = let
-    val (v,x) = dest_abs tm
-    val (s,ty) = dest_var v
-    val new_s = snd (first (fn (z,_) => z = s) ks)
-    in ALPHA_CONV (mk_var(new_s,ty)) tm end handle HOL_ERR _ => NO_CONV tm
-  val th = CONV_RULE (DEPTH_CONV rename_bound_conv) th
-  val th = CONV_RULE ((RATOR_CONV o RAND_CONV) EVAL) th
-  val th = MP th TRUTH
-  in th end;
-
-(*
-val tm = (!last_fail)
-val tm = rhs
-val original_tm = tm
-val tm = dest_conj hyps |> snd |> strip_forall |> snd |> dest_imp |> snd |> rator |> rand |> rand |> rand |> strip_abs |> snd |> rand
-val tm = ``st_ex_return v1``
-
-val tm = dest_conj hyps |> snd
-*)
-fun inst_case_thm tm m2deep = let
-  val tm = if can dest_monad_type (type_of tm) then (inst_monad_type tm) else tm
-  val th = inst_case_thm_for tm
-  val th = CONV_RULE (RATOR_CONV (PURE_REWRITE_CONV [CONJ_ASSOC])) th
-  val (hyps,rest) = dest_imp (concl th)
-  fun list_dest_forall tm = let
-    val (v,tm) = dest_forall tm
-    val (vs,tm) = list_dest_forall tm
-    in (v::vs,tm) end handle HOL_ERR _ => ([],tm)
-  fun take n xs = List.take(xs, n)
-  fun sat_hyp tm = let
-    val (vs,x) = list_dest_forall tm
-    val (x,y) = dest_imp x
-    val z = get_Eval_arg y
-    val lemma = if can dest_monad_type (type_of z)
-                then m2deep z
-                else hol2deep z
-    val lemma = D lemma
-    val new_env = get_Eval_env y
-    val env = env_tm
-    val lemma = INST [env|->new_env] lemma
-    val (x1,x2) = dest_conj x handle HOL_ERR _ => (T,x)
-    val (z1,z2) = dest_imp (concl lemma)
-    val thz =
-      QCONV (SIMP_CONV std_ss [ASSUME x1,Eval_Var_SIMP] THENC
-             ONCE_REWRITE_CONV [EvalM_Var_SIMP] THENC
-             ONCE_REWRITE_CONV [EvalM_Var_SIMP] THENC
-             REWRITE_CONV [lookup_cons_write,lookup_var_write] THENC
-             DEPTH_CONV stringLib.string_EQ_CONV THENC
-             SIMP_CONV std_ss []) z1 |> DISCH x1
-    val lemma = MATCH_MP sat_hyp_lemma (CONJ thz lemma)
-    val bs = take (length vs div 2) vs
-    fun LIST_UNBETA_CONV [] = ALL_CONV
-      | LIST_UNBETA_CONV (x::xs) =
-          UNBETA_CONV x THENC RATOR_CONV (LIST_UNBETA_CONV xs)
-    val lemma = CONV_RULE ((RATOR_CONV o RAND_CONV o RAND_CONV)
-                  (LIST_UNBETA_CONV (rev bs))) lemma
-    val lemma = GENL vs lemma
-    val _ = can (match_term tm) (concl lemma) orelse failwith("sat_hyp failed")
-    in lemma end handle HOL_ERR _ => (print ((term_to_string tm) ^ "\n\n"); last_fail := tm; fail())
-  fun sat_hyps tm = if is_conj tm then let
-    val (x,y) = dest_conj tm
-    in CONJ (sat_hyps x) (sat_hyps y) end else sat_hyp tm
-  val lemma = sat_hyps hyps
-  val th = MATCH_MP th lemma
-  val th = CONV_RULE (RATOR_CONV (DEPTH_CONV BETA_CONV THENC
-                                  REWRITE_CONV [])) th
-  in th end handle Empty => failwith "empty";
-
-(* PMATCH *)
-
-val IMP_EQ_T = Q.prove(`a ==> (a <=> T)`,fs [])
-
-(* DEBUG *)
-val prove_EvalMPatBind_fail = ref T;
-(* END DEBUG *)
-
-fun prove_EvalMPatBind goal m2deep = let
-  val (vars,rhs_tm) = repeat (snd o dest_forall) goal
-                      |> rand |> get_Eval_arg |> rator
-                      |> dest_pabs
-  val res = m2deep rhs_tm
-  val exp = res |> concl |> get_Eval_exp
-  val th = D res
-  val var_assum = ``Eval env (Var n) (a (y:'a))``
-  val is_var_assum = can (match_term var_assum)
-  val vs = find_terms is_var_assum (concl th |> remove_Eval_storePred)
-  fun delete_var tm =
-    if mem tm vs then MATCH_MP IMP_EQ_T (ASSUME tm) else NO_CONV tm
-  val th = CONV_RULE ((RATOR_CONV) (DEPTH_CONV delete_var)) th
-  val th = CONV_RULE ((RATOR_CONV o RAND_CONV)
-              (PairRules.UNPBETA_CONV vars)) th
-  val p = th |> concl |> dest_imp |> fst |> rator
-  val p2 = goal |> dest_forall |> snd |> dest_forall |> snd
-                |> dest_imp |> fst |> rand |> rator
-  val ws = free_vars vars
-  val vs = filter (fn tm => not (mem (rand (rand tm)) ws)) vs |> mk_set
-  val new_goal = goal |> subst [``e:exp``|->exp,p2 |-> p]
-  val new_goal = foldr mk_imp new_goal vs
-  (*
-    set_goal([],new_goal)
-  *)
-  val th = TAC_PROOF (([],new_goal),
-    NTAC (length vs) STRIP_TAC \\ STRIP_TAC
-    \\ fs [FORALL_PROD] \\ REPEAT STRIP_TAC
-    \\ MATCH_MP_TAC (D res) \\ fs []
-    \\ fs [EvalPatBind_def,Pmatch_def]
-    \\ REPEAT (POP_ASSUM MP_TAC)
-    \\ NTAC (length vs) STRIP_TAC
-    \\ CONV_TAC ((RATOR_CONV o RAND_CONV) EVAL)
-    \\ STRIP_TAC \\ fs [] \\ rfs []
-    \\ fs [Pmatch_def,PMATCH_option_case_rwt]
-    (*
-    \\ TRY (SRW_TAC [] [Eval_Var_SIMP,Once EvalM_Var_SIMP,PreImp_def]
-      \\ SRW_TAC [] [Eval_Var_SIMP,Once EvalM_Var_SIMP]
-      \\ EVAL_TAC \\ NO_TAC)
-      *)
-    \\ BasicProvers.EVERY_CASE_TAC \\ fs []
-    \\ rpt (CHANGED_TAC(SRW_TAC [] [Eval_Var_SIMP,Once EvalM_Var_SIMP,lookup_cons_write,lookup_var_write]))
-    \\ TRY (first_x_assum match_mp_tac >> METIS_TAC[])
-    \\ fs[GSYM FORALL_PROD]
-    \\ EVAL_TAC)
-  in UNDISCH_ALL th end handle HOL_ERR e =>
-  (prove_EvalMPatBind_fail := goal;
-   failwith "prove_EvalMPatBind failed");
-
-(* DEBUG *)
-val pmatch_m2deep_fail = ref T;
-val tm = !pmatch_m2deep_fail;
-(* END DEBUG *)
-
-fun pmatch_m2deep tm m2deep = let
-  val (x,ts) = dest_pmatch_K_T tm
-  val v = genvar (type_of x)
-  val x_res = hol2deep x |> D
-  val x_type = type_of x
-  val x_inv = get_type_inv x_type
-  val pmatch_type = type_of tm
-  val pmatch_inv = get_m_type_inv pmatch_type
-  val x_exp = x_res |> UNDISCH |> concl |> rator |> rand
-  val nil_lemma = EvalM_PMATCH_NIL
-		  |> ISPEC H
-                  |> ISPEC pmatch_inv
-                  |> ISPEC x_exp
-                  |> ISPEC v
-                  |> ISPEC x_inv
-  val cons_lemma = EvalM_PMATCH
-		   |> ISPEC H
-                   |> ISPEC pmatch_inv
-                   |> ISPEC x_inv
-                   |> ISPEC x_exp
-                   |> ISPEC v
-  fun prove_hyp conv th =
-    MP (CONV_RULE ((RATOR_CONV o RAND_CONV) conv) th) TRUTH
-  val assm = nil_lemma |> concl |> dest_imp |> fst
-  fun trans [] = nil_lemma
-    | trans ((pat,rhs_tm)::xs) = let
-    (*
-    val ((pat,rhs_tm)::xs) = List.drop(ts,1)
-    val ((pat,rhs_tm)::xs) = ts
-    *)
-    val th = trans xs
-    val p = pat |> dest_pabs |> snd |> hol2deep
-                |> concl |> rator |> rand |> to_pattern
-    val lemma = cons_lemma |> Q.GEN `p` |> ISPEC p
-    val lemma = prove_hyp EVAL lemma
-    val lemma = lemma |> Q.GEN `pat` |> ISPEC pat
-    val lemma = prove_hyp (SIMP_CONV (srw_ss()) [FORALL_PROD]) lemma
-    val lemma = UNDISCH lemma
-    val th = UNDISCH th
-             |> CONV_RULE ((RATOR_CONV o RAND_CONV) (UNBETA_CONV v))
-    val th = MATCH_MP lemma th
-    val th = remove_primes th
-    val goal = fst (dest_imp (concl th))
-    val th = MP th (prove_EvalPatRel goal hol2deep)
-    val th = remove_primes th
-    val th = th |> Q.GEN `res` |> ISPEC rhs_tm
-    val goal = fst (dest_imp (concl th))
-    val th = MATCH_MP th (prove_EvalMPatBind goal m2deep)
-    val th = remove_primes th
-    val th = CONV_RULE ((RATOR_CONV o RAND_CONV)
-          (SIMP_CONV std_ss [FORALL_PROD,patternMatchesTheory.PMATCH_ROW_COND_def])) th
-    val th = DISCH assm th
-    in th end
-  val th = trans ts
-  val th = MATCH_MP th (UNDISCH x_res)
-  val th = UNDISCH_ALL th
-  in th end handle HOL_ERR e =>
-  (pmatch_m2deep_fail := tm;
-   failwith ("pmatch_m2deep failed (" ^ #message e ^ ")"));
-
-(* ---- *)
-
-fun inst_EvalM_env v th = let
-  val thx = th
-  val name = fst (dest_var v)
-  val str = stringLib.fromMLstring name
-  val inv = smart_get_type_inv (type_of v)
-  val tys = Type.match_type (type_of v) (type_of inv |> dest_type |> snd |> List.hd)
-  val v = Term.inst tys v
-  val ri = mk_comb(inv, v)
-  val assum = ``Eval env (Var (Short ^str)) ^ri``
-  val new_env = ``write ^str (v:v) ^env_tm``
-  val old_env = new_env |> rand
-  val th = thx |> UNDISCH_ALL |> REWRITE_RULE [GSYM SafeVar_def]
-               |> DISCH_ALL |> DISCH assum |> SIMP_RULE bool_ss []
-               |> INST [old_env|->new_env]
-               |> SIMP_RULE bool_ss [Eval_Var_SIMP,lookup_var_write]
-               |> ONCE_REWRITE_RULE [EvalM_Var_SIMP]
-               |> ONCE_REWRITE_RULE [EvalM_Var_SIMP]
-               |> REWRITE_RULE [lookup_cons_write,lookup_var_write]
-               |> CONV_RULE (DEPTH_CONV stringLib.string_EQ_CONV)
-               |> SIMP_RULE bool_ss [SafeVar_def]
-  val new_assum = fst (dest_imp (concl th))
-  val th1 = th |> UNDISCH_ALL
-               |> CONV_RULE ((RATOR_CONV o RAND_CONV o RAND_CONV) (UNBETA_CONV v))
-               |> DISCH new_assum
-  in th1 end;
-
-(*
-val v = List.hd l
-val fix = true
-apply_EvalM_Fun (List.hd l) th true
-*)
-(* MATCH_MP th1 th2 fails when:
-   th1 = `!y. (!x. P x y) ==> Q
-   th2 = `!x. P x (f x)`
-   because of name conflicts.
-   MATCH_MP_ABS_RENAME renames the abstractions in th1 to prevent that from happening.
- *)
-(* fun MATCH_MP_FORALL_RENAME th1 th2 =
-  let
-      val th1_hyp = ISPEC H EvalM_Fun_Eq |> concl |> dest_imp |> fst |> strip_forall |> snd
-      (* val (quant_vars, th1_spec_hyp) = strip_forall th1_hyp *)
-      val (tms, tys) = match_term th1_hyp (concl th2);
-      val fvs = FVL (concl (SPEC_ALL th2)::(List.map (fn {redex = _, residue = x} => x) tms)) empty_varset
-      val fvl = HOLset.listItems fvs
-
-      fun rename_foralls_conv fvl tm =
-	if is_forall tm then let
-	    val (x, tm') = dest_forall tm
-  	    val x' = variant fvl x
-	    val conv_f = RAND_CONV ((ABS_CONV (rename_foralls_conv (x'::fvl))) THENC (ALPHA_CONV x'))
-	in
-	    conv_f tm
-	end
-	else REFL tm
-      val ren_th1 = CONV_RULE ((RATOR_CONV o RAND_CONV) (rename_foralls_conv fvl)) th1
-      val subst_th1 = Thm.INST tms (Thm.INST_TYPE tys ren_th1)
-  in
-      MP subst_th1 th2
-  end*)
-
-fun apply_EvalM_Fun v th fix = let
-  val th1 = inst_EvalM_env v th
-  val th2 = if fix then MATCH_MP (ISPEC H EvalM_Fun_Eq) (GEN ``v:v`` th1)
-                   else MATCH_MP (ISPEC H EvalM_Fun) (GEN ``v:v`` (FORCE_GEN v th1))
-  in th2 end;
-
-(* val th1 = (ISPEC H EvalM_Fun_Eq);
-val th2 = (GEN ``v:v`` (inst_EvalM_env v th));
-MATCH_MP_FORALL_RENAME (ISPEC H EvalM_Fun_Eq) (GEN ``v:v`` (inst_EvalM_env v th)) *)
-
-(*
-apply_EvalM_Recclosure fname v th
-
-type_of inv
-type_of v
-*)
-
-fun apply_EvalM_Recclosure fname v th = let
-  val vname = fst (dest_var v)
-  val vname_str = stringLib.fromMLstring vname
-  val fname_str = stringLib.fromMLstring fname
-  val body = th |> UNDISCH_ALL |> concl |> rator |> rator |> rand (* |> concl |> rator |> rand *)
-  val inv = smart_get_type_inv (type_of v)
-  val new_env = ``write ^vname_str v (write_rec
-                    [(^fname_str,^vname_str,^body)] env env)``
-  val old_env = env_tm
-  val tys = Type.match_type (type_of v) (type_of inv |> dest_type |> snd |> List.hd)
-  val v = Term.inst tys v
-  val assum = subst [old_env|->new_env]
-              ``Eval env (Var (Short ^vname_str)) (^inv ^v)``
-  val thx = th |> UNDISCH_ALL |> REWRITE_RULE [GSYM SafeVar_def]
-               |> DISCH_ALL |> DISCH assum |> SIMP_RULE bool_ss []
-               |> INST [old_env|->new_env]
-               |> SIMP_RULE bool_ss [Eval_Var_SIMP]
-               |> ONCE_REWRITE_RULE [EvalM_Var_SIMP]
-               |> ONCE_REWRITE_RULE [EvalM_Var_SIMP]
-               |> REWRITE_RULE [lookup_cons_write,lookup_var_write,write_rec_one]
-               |> CONV_RULE (DEPTH_CONV stringLib.string_EQ_CONV)
-               |> REWRITE_RULE [GSYM write_rec_one]
-               |> SIMP_RULE bool_ss [SafeVar_def]
-  val new_assum = fst (dest_imp (concl thx))
-  val th1 = thx |> UNDISCH_ALL
-                |> CONV_RULE ((RATOR_CONV o RAND_CONV o RAND_CONV) (UNBETA_CONV v)) (* RATOR_CONV *)
-                |> DISCH new_assum
-  val th2 = MATCH_MP (ISPEC H EvalM_Recclosure) (Q.INST [`env`|->`cl_env`] (GEN ``v:v`` th1))
-  val assum = ASSUME (fst (dest_imp (concl th2)))
-  val th3 = D th2 |> REWRITE_RULE [assum]
-  val lemma = MATCH_MP Eval_Eq_Recclosure assum
-  val lemma_lhs = lemma |> concl |> dest_eq |> fst
-  fun replace_conv tm = let
-    val (i,t) = match_term lemma_lhs tm
-    in INST i (INST_TYPE t lemma) end handle HOL_ERR _ => NO_CONV tm
-  val th4 = CONV_RULE (QCONV (DEPTH_CONV replace_conv)) th3
-  in th4 end;
-
-(* Copy-paste from ml_translatorLib *)
-(* check_inv "failwith" tm result DEBUG
-val name = "failwith" *)
-val check_inv_fail = ref T;
-
-fun check_inv name tm result = let
-  val tm2 = get_Eval_arg (concl result)
-  in if aconv tm2 tm then result else let
-    val _ = (check_inv_fail := tm)
-    val _ = (show_types_verbosely := true)
-    val _ = print ("\n\nhol2deep failed at '" ^ name ^ "'\n\ntarget:\n\n")
-    val _ = print_term tm
-    val _ = print "\n\nbut derived:\n\n"
-    val _ = print_term tm2
-    val _ = print "\n\n\n"
-    val _ = (show_types_verbosely := false)
-    in failwith("checkinv") end end
-
-(* end of copy-paste *)
-				   
-(* ---- *)
-
-fun var_hol2deep tm =
-  if is_var tm andalso can get_arrow_type_inv (type_of tm) then let
-    val (name,ty) = dest_var tm
-    val inv = get_arrow_type_inv ty
-    val inv = ONCE_REWRITE_CONV [ArrowM_def] inv |> concl |> rand |> rand
-    val str = stringSyntax.fromMLstring name
-    val result = ASSUME (mk_comb(``Eval env (Var (Short ^str))``,mk_comb(inv,tm)))
-    in check_inv "var" tm result end
-  else hol2deep tm;
-
-(* TODO: automate *)
-val read_refs =
-  [(``get_the_type_constants``,``the_type_constants``,get_the_type_constants_thm),
-   (``get_the_term_constants``,``the_term_constants``,get_the_term_constants_thm),
-   (``get_the_axioms``,``the_axioms``,get_the_axioms_thm),
-   (``get_the_context``,``the_context``,get_the_context_thm)];
-
-val write_refs =
-  [(``set_the_type_constants x``,``the_type_constants``,set_the_type_constants_thm),
-   (``set_the_term_constants x``,``the_term_constants``,set_the_term_constants_thm),
-   (``set_the_axioms x``,``the_axioms``,set_the_axioms_thm),
-   (``set_the_context x``,``the_context``,set_the_context_thm)];
-
-(*
-val tm = rhs
-val tm = !last_m2deep_tm
-*)
-
-(* DEBUG *)
-val last_m2deep_tm = ref ``T``;
-(* END DEBUG *)
-
-(*
-val tm = x1
-val tm = f
-*)
-
-(* DEBUG *)
-fun print_tm_msg msg tm =
-  print (msg  ^(term_to_string tm) ^ "\n\n");
-(* END DEBUG *)
-
-(*
-val tm = rhs
-val tm = ``v5 : 'b -> 'a holKernel$M``
-val tm = ``list_CASE l (ex_return 128) (\x y. ex_return 256)``
-val tm = z
-val tm = concl def |> dest_forall |> snd |> rand |> rand |> dest_abs |> snd |> rator |> rator
-val tm = ``raise_clash v1 : term holKernel$M``
-
-match_term ``(st_ex_return x): ^aM`` tm
-dest_type (type_of tm)
-val tm = ``(st_ex_return v1) : 'b holKernelPmatch$M``
- *)
-
-(* val tm = map_term; *)
-exception BREAKPOINT of term;
-
-fun m2deep tm =
-  (* variable *)
-  if is_var tm then let
-    val _ = print_tm_msg "is_var\n" tm (* DEBUG *)
-    val (name,ty) = dest_var tm
-    val inv = get_arrow_type_inv ty
-    val inv = ONCE_REWRITE_CONV [ArrowM_def] inv |> concl |> rand |> rand
-    val str = stringSyntax.fromMLstring name
-    val result = ASSUME (mk_comb(``Eval env (Var (Short ^str))``,mk_comb(inv,tm)))
-    val result = MATCH_MP (ISPEC H Eval_IMP_PURE) result |> RW [GSYM ArrowM_def]
-    in check_inv "var" tm result end else
-  (* failwith *)
-  if can (match_term ``(failwith s): ^aM``) tm then let
-    val _ = print_tm_msg "failwith\n" tm (* DEBUG *)
-    val ty = dest_monad_type (type_of tm)
-    val inv = smart_get_type_inv (#2 ty) (* fst ty *)
-    val th = hol2deep (rand tm)
-    val asms = List.mapPartial (Lib.total DECIDE) (hyp th)
-    val th = List.foldl (Lib.uncurry PROVE_HYP) th asms
-    val result = ISPEC_EvalM EvalM_failwith |> SPEC (rand tm) |> ISPEC inv
-                 |> UNDISCH |> Lib.C MATCH_MP th
-    in check_inv "failwith" tm result end else
-  (* raise_clash *)
-  if can (match_term ``(raise_clash t): ^aM``) tm then let
-    val _ = print_tm_msg "raise clash\n" tm (* DEBUG *)
-    val ty = dest_monad_type (type_of tm)
-    val inv = smart_get_type_inv (#2 ty) (* fst ty *)
-    val th = hol2deep (rand tm)
-    val result = ISPEC_EvalM EvalM_raise_clash |> SPEC (rand tm) |> ISPEC inv
-                 |> UNDISCH |> Lib.C MATCH_MP th
-    in check_inv "raise_clash" tm result end
-  (* return *)
-  else if can (match_term ``(st_ex_return x): ^aM``) tm then let
-    val _ = print_tm_msg "return\n" tm (* DEBUG *)
-    val th = hol2deep (rand tm)
-    val result = MATCH_MP (ISPEC_EvalM_MONAD EvalM_return) th
-    in check_inv "return" tm result end
-  (* bind *)
-  else if can (match_term ``(st_ex_bind (x:^bM) f): ^aM``) tm then let
-    val _ = print_tm_msg "bind\n" tm (* DEBUG *)
-    val x1 = tm |> rator |> rand
-    val (v,x2) = tm |> rand |> dest_abs
-    val th1 = m2deep x1
-    val th2 = m2deep x2
-    val th2 = inst_EvalM_env v th2
-    val vs = th2 |> concl |> dest_imp |> fst
-    val th2 = th2 |> GEN (rand vs) |> FORCE_GEN (rand (rator vs))
-    val result = MATCH_MP (ISPEC_EvalM_MONAD EvalM_bind) (CONJ th1 th2)
-    in check_inv "bind" tm result end else
-  (* otherwise *)
-  if can (match_term ``(x: ^aM) otherwise (y: ^aM)``) tm then let
-    val _ = print_tm_msg "otherwise\n" tm (* DEBUG *)
-    val x = tm |> rator |> rand
-    val y = tm |> rand
-    val th1 = m2deep x
-    val th2 = m2deep y
-    val th2 = th2 |> DISCH_ALL |> Q.INST [`env`|->`write "v" i env`]
-                  |> REWRITE_RULE [Eval_Var_SIMP2,lookup_cons_write]
-                  |> ONCE_REWRITE_RULE [EvalM_Var_SIMP]
-                  |> ONCE_REWRITE_RULE [EvalM_Var_SIMP]
-                  |> REWRITE_RULE [lookup_cons_write,lookup_var_write]
-                  |> CONV_RULE (DEPTH_CONV stringLib.string_EQ_CONV)
-                  |> REWRITE_RULE []
-                  |> UNDISCH_ALL |> Q.GEN `i`
-    val lemma = Q.SPEC `"v"` (ISPEC_EvalM_MONAD EvalM_otherwise)
-    val result = MATCH_MP (MATCH_MP lemma th1) th2
-    in check_inv "otherwise" tm result end else
-  (* handle_clash *)
-  if can (match_term ``handle_clash (x: ^aM) y``) tm then let
-    val _ = print_tm_msg "handle clash\n" tm (* DEBUG *)
-    val x = tm |> rator |> rand
-    val (v,y) = tm |> rand |> dest_abs
-    val th1 = m2deep x
-    val th2 = m2deep y
-    val th3 = inst_EvalM_env v th2 |> Q.GEN`v` |> FORCE_GEN v
-    val lemma = ISPEC H EvalM_handle_clash |> SPEC_ALL |> UNDISCH
-    val th4 = MATCH_MP lemma th1
-    val result = MATCH_MP th4 th3 handle HOL_ERR _ => HO_MATCH_MP th4 th3
-    in check_inv "handle_clash" tm result end else
-  (* try *)
-  if can (match_term ``try (f:'a-> ^bM) x msg``) tm then let
-    val _ = print_tm_msg "try\n" tm (* DEBUG *)
-    val lemma = tm |> SIMP_CONV (srw_ss()) [try_def]
-    val th = m2deep (lemma |> concl |> rand)
-    val result = th |> RW [GSYM lemma]
-    in check_inv "try" tm result end else
-  (* IGNORE_BIND *)
-  if can (match_term ``IGNORE_BIND (f:'a -> 'b # 'a) (g:'a -> 'c # 'a)``) tm then let
-    val _ = print_tm_msg "IGNORE_BIND\n" tm (* DEBUG *)
-    val lemma = tm |> SIMP_CONV std_ss [state_transformerTheory.IGNORE_BIND_DEF]
-    val th = m2deep (lemma |> concl |> rand)
-    val result = th |> RW [GSYM lemma]
-    in check_inv "IGNORE_BIND" tm result end else
-  (* abs *)
-  if is_abs tm then let
-    val _ = print_tm_msg "abs\n" tm (* DEBUG *)
-    val (v,x) = dest_abs tm
-    val thx = m2deep x
-    val result = apply_EvalM_Fun v thx false
-    in check_inv "abs" tm result end else
-  (* let expressions *)
-  if can dest_let tm andalso is_abs (fst (dest_let tm)) then let
-    val _ = print_tm_msg "let expressions\n" tm (* DEBUG *)
-    val (x,y) = dest_let tm
-    val (v,x) = dest_abs x
-    val th1 = hol2deep y
-    val th2 = m2deep x
-    val th2 = inst_EvalM_env v th2
-    val th2 = th2 |> GEN ``v:v``
-    val z = th1 |> concl |> rand |> rand
-    val th2 = INST [v|->z] th2
-    val result = MATCH_MP (ISPEC H EvalM_Let) (CONJ th1 th2)
-    in check_inv "let" tm result end else
-  (* data-type pattern-matching *)
-  (print_tm_msg "data-type pattern-matching\n" tm (* DEBUG *); inst_case_thm tm m2deep) handle HOL_ERR _ =>
-  (* previously translated term *) 
-  if can lookup_v_thm tm then let
-    val _ = print_tm_msg "previously translated\n" tm (* DEBUG *)
-    val th = lookup_v_thm tm
-    val inv = smart_get_type_inv (type_of tm)
-    val target = mk_comb(inv,tm)
-    val (ss,ii) = match_term (th |> concl |> rand) target
-    val result = INST ss (INST_TYPE ii th)
-                 |> MATCH_MP (ISPEC H Eval_IMP_PURE)
-                 |> REWRITE_RULE [GSYM ArrowM_def]
-    in check_inv "lookup_v_thm" tm result end else
-  (* if *)
-  if can (match_term ``if b then x: ^aM else y: ^aM``) tm then let
-    val _ = print_tm_msg "if\n" tm (* DEBUG *)
-    val (t,x1,x2) = dest_cond tm
-    val th0 = hol2deep t
-    val th1 = m2deep x1
-    val th2 = m2deep x2
-    val th = MATCH_MP (ISPEC H EvalM_If) (LIST_CONJ [D th0, D th1, D th2])
-    val result = UNDISCH th
-    in check_inv "if" tm result end else
-  (* ref: get_the_(...) *)
-  if can (first (fn (t,_,_) => same_const t tm)) read_refs then let
-    val _ = print_tm_msg "ref get_the(...)\n" tm (* DEBUG *)
-    val (_,t,result) = first (fn (t,_,_) => same_const t tm) read_refs
-    val result = result |> UNDISCH_ALL
-    in check_inv "get" tm result end else
-  (* ref: set_the_(...) *)
-  if can (first (fn (t,_,_) => can (match_term t) tm)) write_refs then let
-    val _ = print_tm_msg "ref: set_the(...)\n" tm (* DEBUG *)
-    val (_,t,result) = (first (fn (t,_,_) => can (match_term t) tm)) write_refs
-    val th = result |> UNDISCH
-    val result = MATCH_MP th (hol2deep (tm |> rand))
-    in check_inv "set" tm result end else
-  (* recursive pattern *)
-  if can match_rec_pattern tm then let
-    val _ = print_tm_msg "recursive pattern\n" tm (* DEBUG *)
-    val (lhs,fname,pre_var) = match_rec_pattern tm
-    fun dest_args tm = rand tm :: dest_args (rator tm) handle HOL_ERR _ => []
-    val xs = dest_args tm
-    val f = repeat rator lhs
-    val str = stringLib.fromMLstring fname
-    fun mk_fix tm = let
-      val inv_type = type_of tm
-      val inv = smart_get_type_inv inv_type
-      val eq = ``Eq ^inv ^tm``
-      (* TODO: move that *)
-      val PURE_tm = Term.inst [``:'a`` |-> inv_type, ``:'b`` |-> refs_type] ``PURE : ('a -> v -> bool) -> ('a, 'b) H``
-      in ``^PURE_tm (Eq ^inv ^tm)`` end
-    fun mk_m_arrow x y = ``ArrowM ^H ^x ^y``
-    fun mk_inv [] res = res
-      | mk_inv (x::xs) res = mk_inv xs (mk_m_arrow (mk_fix x) res)
-(*
-val x = hd xs
-val res = (get_m_type_inv (type_of tm))
-val ty = type_of tm
-*)
-    val inv = mk_inv xs (get_m_type_inv (type_of tm))
-    val ss = fst (match_term lhs tm)
-    val pre = T (* subst ss (rec_pre_var ()) *)
-    val tys = match_type (type_of f) (type_of inv |> dest_type |> snd |> List.hd)
-    val f' = Term.inst tys f
-    val h = ASSUME ``PreImp ^pre (EvalM env (Var (Short ^str)) (^inv ^f') ^H)``
-            |> RW [PreImp_def] |> UNDISCH
-(*
-val original_tm
-val tm = List.last xs
-*)
-    val ys = map (fn tm => MATCH_MP (ISPEC H Eval_IMP_PURE)
-                             (MATCH_MP Eval_Eq (var_hol2deep tm))) xs
-    fun apply_arrow hyp [] = hyp
-      | apply_arrow hyp (x::xs) =
-          MATCH_MP (MATCH_MP (ISPEC H EvalM_ArrowM) (apply_arrow hyp xs)) x
-          (* MATCH_MP (MATCH_MP EvalM_ArrowM (apply_arrow hyp xs)) x *)
-    val result = apply_arrow h ys
-    in check_inv "rec_pattern" tm result end else
-  (* PMATCH *)
-  if is_pmatch tm then let
-    val _ = print_tm_msg "PMATCH\n" tm (* DEBUG *)
-    val original_tm = tm
-    val lemma = pmatch_preprocess_conv tm
-    val tm = lemma |> concl |> rand
-    val result = pmatch_m2deep tm m2deep
-    val result = result |> CONV_RULE (RATOR_CONV (RAND_CONV (RAND_CONV (K (GSYM lemma)))))
-    in check_inv "pmatch_m2deep" original_tm result end else
-  (* normal function applications *)
-  if is_comb tm then let
-    val _ = print_tm_msg "normal function application\n" tm (* DEBUG *)
-    val (f,x) = dest_comb tm
-    val thf = m2deep f
-    val result = hol2deep x |> MATCH_MP (ISPEC H Eval_IMP_PURE)
-                            |> MATCH_MP (MATCH_MP (ISPEC H EvalM_ArrowM) thf)
-                 handle e =>
-                 m2deep x |> MATCH_MP (MATCH_MP (ISPEC H EvalM_ArrowM) thf)
-    in check_inv "comb" tm result end else
-  (last_m2deep_tm := tm; failwith ("cannot translate: " ^ term_to_string tm));
-
-fun get_curr_prog_state () = let
-  val k = ref init_state
-  val _ = ml_prog_update (fn s => (k := s; s))
-  in !k end
-
-(*
-val def = FST;
-val def = !last_def;
-val def = map_def;
-val assoc_conv_tm = th |> concl |> rand |> rator |> rand
-*)
-fun EvalM_P_CONV CONV tm =
-  if is_imp tm then (RAND_CONV o RATOR_CONV o RAND_CONV) CONV tm
-  else (RATOR_CONV o RAND_CONV) CONV tm;
-
-(* DEBUG *)
-val last_def = ref assoc_def;
-(* END DEBUG *)
-
-(* Performs a conversion of the form: (\x. M x) = M *)
-(* fun ABS_PREDICATE_CONV tm =
-  if is_abs tm then let
-      val (x, body) = dest_abs tm
-      val P = rator body
-      val spec_ETA_THM = ISPEC P ETA_THM
-  in spec_ETA_THM end
-  handle HOL_ERR _ => raise (ERR "ABS_PREDICATE_CONV" "not valid term")
-  else raise (ERR "ABS_PREDICATE_CONV" "not valid term"); *)
-				 
-fun m_translate def = let
-  val original_def = def
-  (* DEBUG *)
-  val _ = (last_def := original_def)			 
-  (* END DEBUG *)
-  fun the (SOME x) = x | the _ = failwith("the of NONE")
-  (* perform preprocessing -- reformulate def *)
-  val (is_rec,defs,ind) = preprocess_def def
-  val _ = length defs = 1 orelse failwith "no support for mutual recursion"
-  val def = hd defs
-  val (lhs,rhs) = dest_eq (concl def)
-  val fname = repeat rator lhs |> dest_const |> fst |> get_unique_name
-  val _ = print ("Translating monadic " ^ fname ^ "\n")
-  val fname_str = stringLib.fromMLstring fname
-  (* read off information *)
-  (* val _ = register_term_types (concl def) *)
-  fun rev_param_list tm = rand tm :: rev_param_list (rator tm) handle HOL_ERR _ => []
-  val rev_params = def |> concl |> dest_eq |> fst |> rev_param_list
-  val no_params = (length rev_params = 0)
-  (* derive deep embedding *)
-  val rhs = if can dest_monad_type (type_of rhs) then inst_monad_type rhs else rhs
-  val _ = install_rec_pattern lhs fname fname
-  val th = m2deep rhs
-  val _ = uninstall_rec_patterns ()
-  (* replace rhs with lhs in th *)
-  val th = CONV_RULE (EvalM_P_CONV (* Prev : RAND_CONV o RAND_CONV *)
-             (REWRITE_CONV [CONTAINER_def] THENC ONCE_REWRITE_CONV [GSYM def])) th
-  (* abstract parameters *)
-  val th = clean_assumptions (D th)
-  val (th,v) = if no_params then (th,T) else
-                 (foldr (fn (v,th) => apply_EvalM_Fun v th true) th
-                    (rev (if is_rec then butlast rev_params else rev_params)),
-                  last rev_params)
-  val th = if not is_rec then D (clean_assumptions th)
-           else apply_EvalM_Recclosure fname v th |> clean_assumptions
-  val th = CONV_RULE (QCONV (DEPTH_CONV ETA_CONV)) th
-  val th = if is_rec then Q.INST [`shaddow_env`|->`cl_env`] th
-                     else Q.INST [`shaddow_env`|->`env`] th
-  val th = th |> REWRITE_RULE [lookup_cons_write]
-  (* collect precondition *)
-  val th = CONV_RULE ((RATOR_CONV o RAND_CONV)
-                      (SIMP_CONV std_ss [EVAL ``CONTAINER TRUE``,
-                                         EVAL ``CONTAINER FALSE``])) th
-  val th = clean_assumptions th
-  val (th,pre) = if no_params then (th,NONE) else
-                  (th |> REWRITE_RULE [PreImp_def,PRECONDITION_def],NONE)
-  (* apply induction *)
-  val th = if not is_rec then th else let
-    val th = REWRITE_RULE [CONTAINER_def, addressTheory.CONTAINER_def] th (* TODO: find why some CONTAINER definitions are taken from address *)
-    val hs = hyp th
-    val hyp_tm = list_mk_abs(rev rev_params, th |> UNDISCH_ALL |> concl)
-    val goal = list_mk_forall(rev rev_params, th |> UNDISCH_ALL |> concl)
-    val goal = mk_imp(list_mk_conj hs,goal)
-    val ind_thm = (the ind)
-    val ind_thm = rename_bound_vars_rule "i" ind_thm
-                  |> SIMP_RULE std_ss []
-(*
-    set_goal([],goal)
-*)
-    val lemma = prove(goal,
-      STRIP_TAC
-      \\ SIMP_TAC std_ss [FORALL_PROD]
-      \\ MATCH_MP_TAC (SPEC hyp_tm ind_thm |> CONV_RULE (DEPTH_CONV BETA_CONV))
-      \\ REPEAT STRIP_TAC \\ MATCH_MP_TAC th
-      \\ FULL_SIMP_TAC (srw_ss()) [ADD1,write_rec_one]
-      \\ REPEAT STRIP_TAC
-      \\ MATCH_MP_TAC IND_HELP
-      \\ Q.EXISTS_TAC `env`
-      \\ ASM_SIMP_TAC std_ss []
-      \\ FULL_SIMP_TAC (srw_ss()) [ADD1]
-      \\ FULL_SIMP_TAC std_ss [UNCURRY_SIMP]
-      \\ METIS_TAC [])
-    val th = UNDISCH lemma |> SPECL (rev rev_params)
-    val th = RW [PreImp_def] th |> UNDISCH_ALL
-    in th end
-  (* remove Eq *)
-  val th = RW [ArrowM_def] th
-  fun update_params_type th params = let
-      val fvs = free_vars (concl th)
-      val tmap = foldl (fn(x, m) => Redblackmap.insert(m, dest_var x |> fst, x))
-                (Redblackmap.mkDict String.compare) fvs
-      val params = List.map (fn x => Redblackmap.find (tmap, dest_var x |> fst)) params
-  in params end
-  val rev_params = update_params_type th rev_params
-  fun f (v,th) =
-    HO_MATCH_MP (ISPEC_EvalM EvalM_FUN_FORALL) (GEN v th) |> SIMP_RULE std_ss [M_FUN_QUANT_SIMP]
-  val th = foldr f th rev_params handle HOL_ERR _ => th
-  val th = RW [GSYM ArrowM_def] th
-  (* simpliy EqualityType *)
-  val th = SIMP_EqualityType_ASSUMS th
-  (* abbreviate code *)
-  val th = th |> DISCH_ALL |> REWRITE_RULE [GSYM AND_IMP_INTRO] |> UNDISCH_ALL
-  val th = RW [ArrowM_def] th
-  val th = if is_rec then let
-      val recc = (first (can (find_term
-                    (fn tm => tm = rator ``Recclosure ^env_tm``)))
-                        (hyp th)) |> rand |> rator |> rand
-      val v_names = map (fn x => find_const_name (x ^ "_v"))
-                      (recc |> listSyntax.dest_list |> fst
-                            |> map (stringSyntax.fromHOLstring o rand o rator))
-      val _ = ml_prog_update (add_Dletrec recc v_names)
-      val s = get_curr_prog_state ()
-      val v_def = hd (get_v_defs s)
-      val cl_env = v_def |> concl |> rand |> rator |> rator |> rand
-      val th = th |> Q.INST [`cl_env`|->`^cl_env`]
-                  |> DISCH_ALL |> REWRITE_RULE [GSYM v_def]
-                  |> clean_assumptions |> DISCH_ALL
-                  |> REWRITE_RULE [GSYM AND_IMP_INTRO] |> UNDISCH_ALL
-      val th = th |> DISCH (first (can (match_term ``LOOKUP_VAR _ _ _``)) (hyp th))
-      val th = MATCH_MP (MP (ISPEC H LOOKUP_VAR_EvalM_IMP) VALID_STORE_THM) (Q.GEN `env` th) (* HERE!! *)
-      in th end
-    else let
-      val th = th |> Q.INST [`env`|->`^(get_env (get_curr_prog_state ()))`]
-                  |> D |> clean_assumptions |> UNDISCH_ALL
-      val th = th |> MATCH_MP (MP (ISPEC H EvalM_Fun_PURE_IMP) VALID_STORE_THM)
-      val v = th |> concl |> rand |> rator |> rand
-      val e = th |> concl |> rand |> rand
-      val v_name = find_const_name (fname ^ "_v")
-      val _ = ml_prog_update (add_Dlet_Fun fname_str v e v_name)
-      val s = get_curr_prog_state ()
-      val v_def = hd (get_v_defs s)
-      val th = th |> REWRITE_RULE [GSYM v_def]
-      in th end
-  val th = RW [GSYM ArrowM_def] th
-  (* store certificate for later use *)
-  val pre = (case pre of NONE => TRUTH | SOME pre_def => pre_def)
-  val _ = add_v_thms (fname,fname,th,pre)
-  val th = save_thm(fname ^ "_v_thm",th)
-  in th end
-    handle UnableToTranslate tm => let
-    val _ = print "\n\nml_translate: cannot translate term:  "
-    val _ = print_term tm
-    val _ = print "\n\nwhich has type:\n\n"
-    val _ = print_type (type_of tm)
-    val _ = print "\n\n"
-    in raise UnableToTranslate tm end
-  (* DEBUG *)
-    | HOL_ERR err => let
-    val _ = print "\n\nml_translate: unexpected error when translating term:\n\n"
-    val _ = print_thm def
-    val _ = print "\n\n"
-    in raise (HOL_ERR err) end;
-
+(**************************************************************************************************)
+(**************************************************************************************************)
 (* --- perform translation --- *)
 
 val res = translate FST;
@@ -1299,12 +437,6 @@ val res = translate holSyntaxTheory.orda_def;
 val res = translate holSyntaxTheory.term_remove_def;
 val res = translate holSyntaxTheory.term_union_def;
 
-(* DEBUG *)
-val def = vsubst_def;
-m_translate def;
-val tm = (def (* rec *) |> m_translate; ``T``) handle BREAKPOINT tm => tm;
-(* END DEBUG *)
-
 val def = assoc_def   (* rec *) |> m_translate
 val def = map_def    (* rec *) |> m_translate
 val def = forall_def (* rec *) |> m_translate
@@ -1381,5 +513,7 @@ val candle_prog_thm =
   |> CONV_RULE ((RAND_CONV)
                 (EVAL THENC define_abbrev_conv "candle_init_state"))
   |> curry save_thm "candle_prog_thm"
+
+val _ = (print_asts := true);
 
 val _ = export_theory();
